proof/refine/X64/ArchAcc_R.thy
@@ -1790,26 +1790,33 @@ lemma asidHighBitsOf [simp]:
   apply (simp add: word_size nth_ucast)
   done
 
-term vspace_at_asid
-
-find_consts "64 word \<Rightarrow> 'a state \<Rightarrow> bool" name:asid
+lemma asidLowBitsOf [simp]:
+  "asidLowBitsOf asid = ucast (asid_low_bits_of asid)"
+  apply (simp add: asidLowBitsOf_def asid_low_bits_of_def asid_low_bits_def)
+  apply (rule word_eqI)
+  apply (simp add: word_size nth_ucast)
+  done
 
 (* FIXME: move to invariants? *)
 definition
   "vspace_at_asid_ex asid \<equiv> \<lambda>s. \<exists>pm. vspace_at_asid asid pm s"
+
+lemma le_mask_asidBits_asid_wf:
+  "asid_wf asid \<longleftrightarrow> asid \<le> mask asidBits"
+  by (simp add: asidBits_def asidHighBits_def asid_wf_def asid_bits_defs mask_def)
 
 lemma find_vspace_for_asid_corres:
   assumes "asid' = asid"
   shows "corres (lfr \<oplus> op =)
                 ((\<lambda>s. valid_arch_state s \<or> vspace_at_asid_ex asid s)
                     and valid_vspace_objs and pspace_aligned
-                    and K (0 < asid \<and> asid \<le> mask asidBits))
+                    and K (0 < asid \<and> asid_wf asid))
                 (pspace_aligned' and pspace_distinct' and no_0_obj')
                 (find_vspace_for_asid asid) (findVSpaceForASID asid')"
   using assms
   apply (simp add: find_vspace_for_asid_def findVSpaceForASID_def)
   apply (rule corres_gen_asm, simp)
-  apply (simp add: liftE_bindE asidRange_def
+  apply (simp add: liftE_bindE asidRange_def le_mask_asidBits_asid_wf
                    mask_2pm1[symmetric])
   apply (rule_tac r'="\<lambda>x y. x = y o ucast"
              in corres_split' [OF _ _ gets_sp gets_sp])
@@ -1835,7 +1842,7 @@ lemma find_vspace_for_asid_corres:
          apply (rule rangeI[where x=0])
         apply simp
        apply clarsimp
-      apply (simp add: mask_asid_low_bits_ucast_ucast returnOk_def
+      apply (simp add: mask_asid_low_bits_ucast_ucast asid_low_bits_of_def returnOk_def
                        lookup_failure_map_def
                 split: option.split)
       apply clarsimp
@@ -1878,7 +1885,7 @@ lemma find_vspace_for_asid_corres':
   assumes "asid' = asid"
   shows "corres (lfr \<oplus> op =)
                 (vspace_at_asid_ex asid and valid_vspace_objs
-                    and pspace_aligned and  K (0 < asid \<and> asid \<le> mask asidBits))
+                    and pspace_aligned and  K (0 < asid \<and> asid_wf asid))
                 (pspace_aligned' and pspace_distinct' and no_0_obj')
                 (find_vspace_for_asid asid) (findVSpaceForASID asid')"
   apply (rule corres_guard_imp, rule find_vspace_for_asid_corres[OF assms])
