proof/refine/X64/Finalise_R.thy
@@ -3735,10 +3735,10 @@ lemma arch_finalise_cap_corres:
       apply (rule corres_guard_imp, rule unmap_page_corres[OF refl refl refl refl])
        apply simp
        apply (clarsimp simp: valid_cap_def valid_unmap_def)
-       apply (auto simp: vmsz_aligned_def pbfs_atleast_pageBits mask_def
+       apply (auto simp: vmsz_aligned_def pbfs_atleast_pageBits mask_def wellformed_mapdata_def
                    elim: is_aligned_weaken)[2]
      apply (rule corres_guard_imp, rule unmap_page_table_corres[OF refl refl refl])
-      apply (auto simp: valid_cap_def valid_cap'_def mask_def bit_simps
+      apply (auto simp: valid_cap_def valid_cap'_def mask_def bit_simps wellformed_mapdata_def
                  elim!: is_aligned_weaken)[2]
     apply (rule corres_guard_imp, rule unmap_pd_corres[OF refl refl refl])
      apply (auto simp: valid_cap_def valid_cap'_def mask_def bit_simps wellformed_mapdata_def
