spec/abstract/MiscMachine_A.thy
@@ -26,12 +26,16 @@ requalify_types
   register
   data
   obj_ref
-  asid_index
-  asid_pool_index
+  asid_high_len
+  asid_high_index
+  asid_low_len
+  asid_low_index
+  asid_len
+  asid_rep_len
+  asid
   cap_ref
   length_type
   vspace_ref
-  data_offset
 
 requalify_consts
   nat_to_cref
@@ -43,7 +47,6 @@ requalify_consts
   gp_registers
   exception_message
   syscall_message
-
   new_context
   slot_bits
   oref_to_data
@@ -54,7 +57,6 @@ requalify_consts
   data_to_nat
   data_to_16
   data_to_cptr
-  data_offset_to_nat
   combine_ntfn_badges
 
 end
@@ -62,5 +64,29 @@ end
 (* Needs to be done here after plain type names are exported *)
 translations
   (type) "'a user_monad" <= (type) "user_context \<Rightarrow> ('a \<times> user_context) set \<times> bool"
+
+definition
+  asid_high_bits :: nat
+where
+  "asid_high_bits \<equiv> LENGTH(asid_high_len)"
+
+definition
+  asid_low_bits :: nat
+where
+  "asid_low_bits \<equiv> LENGTH(asid_low_len)"
+
+definition
+  asid_bits :: nat
+where
+  "asid_bits \<equiv> LENGTH(asid_len)"
+
+lemmas asid_bits_defs =
+  asid_bits_def asid_high_bits_def asid_low_bits_def
+
+(* Sanity checks. *)
+lemma asid_bits_len_checks:
+  "asid_bits = asid_high_bits + asid_low_bits"
+  "asid_bits \<le> LENGTH(asid_rep_len)"
+  unfolding asid_bits_defs by auto
 
 end
